Almost complete proof of wp_mapIter and complete proof of wp_MapDeepEqual

src/iter/map_iter.v
@@ -5,16 +5,19 @@ From New.generatedproof.sys_verif_code Require Import iterator.
 Section proof.
 Context `{hG: !heapGS Σ} `{!globalsGS Σ} {go_ctx: GoContext}.
 
+(* TODO: is it advisable to add the typeclasses for K and V into the context? *)
+Context `{Inhabited K} `{Countable K} `{!IntoVal K} `{!IntoValTyped K kt}.
+Context `{Inhabited V} `{!IntoVal V} `{!IntoValTyped V vt}.
+
 #[global] Instance : IsPkgInit iterator := define_is_pkg_init True%I.
 #[global] Instance : GetIsPkgInitWf iterator := build_get_is_pkg_init_wf.
 
-Definition is_mapIter `{Countable K} `{!IntoVal K} `{!IntoVal V} (mapIter : func.t)
-    (m : gmap K V) (P : gmap K V → iPropI Σ) Φ : iPropI Σ :=
-  ∀ (yield : func.t), (
+Definition is_mapIter (mapIter : func.t) (m : gmap K V) : iPropI Σ :=
+  ∀ (P : gmap K V → iPropI Σ) Φ (yield : func.t), (
     "HP" :: P(∅) ∗
     "#Hyield" :: □(
       ∀ (k : K) (v : V) (sm : gmap K V),
-        (⌜ (<[ k := v ]> sm) ⊆ m ⌝ ∗ P(sm)) -∗
+        (⌜ k ∉ dom sm ∧ (<[ k := v ]> sm) ⊆ m ⌝ ∗ P(sm)) -∗
         WP #yield #k #v {{
           ok,
           if (decide (ok = #true)) then
@@ -29,13 +32,402 @@ Definition is_mapIter `{Countable K} `{!IntoVal K} `{!IntoVal V} (mapIter : func
   )%I -∗
   WP #mapIter #yield {{ _, Φ }}.
 
-Lemma wp_mapIter `{Countable K} `{!IntoVal K} `{!IntoValTyped K kt} `{!IntoVal V} `{!IntoValTyped V vt} 
-    mref (m : gmap K V) P Φ' :
+Axiom wp_map_for_range :
+  ∀ mref (m : gmap K V) (body : func.t) dq Φ,
+  own_map mref dq m ∗
+  (∀ keys_sl keys,
+     ⌜ list_to_set keys = dom m ∧ length keys = size m ∧ NoDup keys ⌝ ∗
+     own_slice keys_sl DfracDiscarded keys -∗
+      WP slice.for_range (#kt) (#keys_sl) (
+          λ: <> "k"%string,
+          let: "kv"%string := (map.get (#mref) "k"%string) in
+          let: "v"%string := Fst "kv"%string in 
+          #body "k"%string ("v"%string)
+      )%E {{ _, own_map mref dq m ∗ Φ }}
+  ) -∗ 
+  WP map.for_range #mref #body {{ _, Φ }}.
+
+(* TODO: what amount of ownership should be given to the iterator? (mirroring concerns about slice iterator) *)
+Lemma wp_mapIter mref (m : gmap K V):
   {{{
     is_pkg_init iterator ∗
     "#Hmap" :: own_map mref DfracDiscarded m
   }}}
     @! iterator.mapIter #kt #vt #mref
-  {{{ (f : func.t), RET #f; is_mapIter f m P Φ' }}}.
+  {{{ (f : func.t), RET #f; is_mapIter f m }}}.
 Proof.
+  wp_start.
+  iNamed "Hpre".
+  wp_auto.
+  iApply "HΦ".
+  clear Φ.
+  unfold is_mapIter.
+  iIntros (P Φ yield) "Hpre".
+  iNamed "Hpre".
+  wp_auto.
+  iPersist "m".
+  wp_bind (map.for_range _ _).
+  iApply (wp_wand with "[HP Htrace yield k v]").
+  {
+    iApply (wp_map_for_range mref m _ DfracDiscarded Φ).
+    iSplitR ; first done.
+    iIntros (keys_sl keys) "[%Hpure #Hkeys]".
+    iDestruct (own_slice_len with "Hkeys") as "[%Hlength %Hslice_len]".
+    destruct Hpure as [Hkeys_m [Hkeys_m_card Hno_dup]].
+    wp_auto.
+    iAssert (
+      ∃(k : K)(v : V)(i : w64)(sm : gmap K V),
+      "k" :: k_ptr ↦ k ∗
+      "v" :: v_ptr ↦ v ∗
+      "i" :: i_ptr ↦ i ∗
+      "HP" :: P(sm) ∗
+      "%Hsm" :: ⌜ ∅ ⊆ sm ⊆ m ⌝ ∗
+      "%Hsm_card" :: ⌜ sint.nat i = size sm ⌝ ∗
+      "%Hsm_dom" :: ⌜ list_to_set (firstn (sint.nat i) keys) = dom sm ⌝ ∗
+      "%Hi" :: ⌜ 0 ≤ sint.Z i ≤ size m ⌝
+    )%I with "[k v i HP]" as "Hinv".
+    {
+      iExists (default_val K), (default_val V), (W64 0), ∅.
+      iFrame.
+      iSplitL.
+      {
+        iPureIntro.
+        split ; first set_solver.
+        apply map_empty_subseteq.
+      }
+      iSplitL.
+      {
+        iPureIntro.
+        replace (sint.nat (W64 0)) with 0%nat by word.
+        set_solver.
+      }
+      iSplitL.
+      {
+        iPureIntro.
+        replace (sint.nat (W64 0)) with 0%nat by word.
+        rewrite firstn_0.
+        set_solver.
+      }
+      word.
+    }
+    wp_for "Hinv".
+    wp_if_destruct.
+    2: {
+      iSplitR ; first done.
+      iApply "Htrace".
+      assert (size sm = size m) as Hsm_m_size by word.
+      assert (sm = m).
+      {
+        apply map_subseteq_size_eq ; [set_solver | lia].
+      }
+      subst.
+      iFrame.
+    }
+    wp_pure ; first word.
+    wp_apply (wp_load_slice_elem _ _ _ _ (keys !!! sint.nat i)) ; first word.
+    {
+      iSplitL ; first done.
+      iPureIntro.
+      rewrite list_lookup_lookup_total_lt ; first word.
+      done.
+    }
+    iIntros "_".
+    wp_auto.
+    wp_apply wp_map_get ; first done.
+    iIntros "_".
+    wp_auto.
+    wp_bind (#yield _ _).
+    replace (m !! (keys !!! sint.nat i)) with (Some (m !!! (keys !!! sint.nat i))).
+    2 : {
+      symmetry.
+      rewrite lookup_lookup_total_dom ; last done.
+      rewrite <- Hkeys_m.
+      rewrite elem_of_list_to_set.
+      apply list_elem_of_lookup_total_2.
+      word.
+    }
+    simpl.
+    assert (take (S (sint.nat i)) keys = take (sint.nat i) keys ++ [keys !!! (sint.nat i)]) as Htake_S.
+    {
+      apply take_S_r.
+      apply list_lookup_lookup_total_lt.
+      word.
+    }
+    (* This should be generalized into its own lemma after replace dom sm, but my attempts were unsuccessful *)
+    assert (keys !!! sint.nat i ∉ dom sm) as Hkeys_not_elem_of.
+    {
+      assert (NoDup (firstn (S (sint.nat i)) keys)) as Hfirstn_keys_NoDup.
+      {
+        pose proof (sublist_take keys (S (sint.nat i))).
+        apply (sublist_NoDup _ keys) ; done.
+      }
+      rewrite Htake_S in Hfirstn_keys_NoDup.
+      apply NoDup_ListNoDup in Hfirstn_keys_NoDup.
+      apply NoDup_remove in Hfirstn_keys_NoDup as [_ Hnot_In].
+      rewrite <- Hsm_dom.
+      apply not_elem_of_list_to_set.
+      unfold not.
+      intros Hkeys_dom.
+      apply Hnot_In.
+      rewrite app_nil_r.
+      apply list_elem_of_In.
+      done.
+    }
+    iApply (wp_wand with "[HP]").
+    {
+      wp_apply ("Hyield" $! _ _ sm).
+      iFrame.
+      iPureIntro.
+      split.
+      - done.
+      - apply insert_subseteq_l ; last set_solver.
+        apply lookup_lookup_total_dom.
+        rewrite <- Hkeys_m.
+        apply elem_of_list_to_set.
+        apply list_elem_of_lookup_total_2.
+        word.
+    }
+    iIntros (?).
+    destruct (decide _).
+    {
+      iIntros "HP".
+      subst.
+      wp_auto.
+      wp_for_post.
+      iFrame.
+      iSplitL.
+      {
+        iPureIntro.
+        split ; first apply map_empty_subseteq.
+        apply insert_subseteq_l ; last set_solver.
+        apply lookup_lookup_total_dom.
+        rewrite <- Hkeys_m.
+        apply elem_of_list_to_set.
+        apply list_elem_of_lookup_total_2.
+        word.
+      }
+      iSplitL.
+      {
+        iPureIntro.
+        replace (sint.nat (word.add _ _)) with (S (sint.nat i)) by word.
+        rewrite map_size_insert.
+        assert (sm !! (keys !!! sint.nat i) = None) as Hsm_lookup_none.
+        {
+          apply not_elem_of_dom.
+          done.
+        }
+        rewrite Hsm_lookup_none.
+        word.
+      }
+      iSplitL.
+      {
+        iPureIntro.
+        replace (sint.nat (word.add _ _)) with (S (sint.nat i)) by word.
+        symmetry.
+        rewrite dom_insert_L.
+        rewrite Htake_S.
+        set_solver.
+      }
+      word.
+    }
+    destruct (decide _).
+    {
+      iIntros "HΦ'".
+      subst.
+      wp_auto.
+      wp_for_post.
+      iFrame.
+      done.
+    }
+    iIntros "?".
+    done.
+  }
+  iIntros (?) "HΦ".
+  wp_auto.
+  (* TODO: why is it stuck? *)
 Admitted.
+
+(* TODO: tried to give this a proof in Perennial, countered by lack of map.for_range spec *)
+Axiom wp_map_len : ∀ l (m : gmap K V) dq,
+  {{{ l ↦${dq} m }}}
+    map.len #l
+  {{{ (s : w64), RET #s; ⌜ sint.Z s = size m ⌝ ∗ l ↦${dq} m }}}.
+
+(* TODO: is this axiom sane? *)
+Axiom wp_interace_eq : ∀ (v1 v2 : V),
+  {{{ True }}}
+    interface.eq (#v1) (#v2)
+  {{{ (b : bool), RET #b; ⌜ b = bool_decide (v1 = v2) ⌝ }}}.
+
+Lemma wp_MapDeepEqual mref1 (m1 : gmap K V) mref2 (m2 : gmap K V) :
+  {{{
+    is_pkg_init iterator ∗
+    "#Hmap1" :: own_map mref1 DfracDiscarded m1 ∗
+    "#Hmap2" :: own_map mref2 DfracDiscarded m2
+  }}}
+    @! iterator.mapDeepEqual #kt #vt #mref1 #mref2
+  {{{
+    (b : bool), RET #b; ⌜ b = bool_decide (m1 = m2) ⌝
+  }}}.
+Proof.
+  wp_start.
+  iNamed "Hpre".
+  wp_auto.
+  iPersist "m1 m2".
+  wp_apply (wp_map_len _ m1) ; first done.
+  iIntros (s1) "[%Hs1 _]".
+  wp_auto.
+  wp_apply (wp_map_len _ m2) ; first done.
+  iIntros (s2) "[%Hs2 _]".
+  wp_auto.
+  wp_if_destruct.
+  2 : {
+    iApply "HΦ".
+    iPureIntro.
+    assert (m1 ≠ m2).
+    {
+      unfold not.
+      intros Heq.
+      assert (size m1 ≠ size m2) as Hsize by word.
+      apply Hsize.
+      rewrite Heq.
+      done.
+    }
+    rewrite bool_decide_eq_false_2 ; done.
+  }
+  wp_apply (wp_mapIter mref1 m1) ; first done.
+  iIntros (f) "HmapIter".
+  wp_auto.
+  unfold is_mapIter.
+  wp_bind (#f _).
+  iApply (wp_wand with "[ret_val HmapIter]").
+  {
+    iApply (
+      "HmapIter" $!
+      (λ m, ret_val_ptr ↦ bool_decide (m ⊆ m2))%I
+      (ret_val_ptr ↦ bool_decide (m1 = m2))%I
+    ).
+    iSplitL.
+    {
+      rewrite bool_decide_eq_true_2 ; [apply map_empty_subseteq | done].
+    }
+    iSplitR.
+    {
+      iModIntro.
+      iIntros (k v sm) "[%Hpure ret_val]".
+      destruct Hpure as [Hk_not_elem_of_sm Hsm_insert_le_m1].
+      wp_auto.
+      wp_apply wp_map_get ; first done.
+      iIntros "_".
+      wp_auto.
+      wp_if_destruct.
+      {
+        wp_if_destruct.
+        - replace (m2 !! k) with (Some v).
+          2 : {
+            symmetry.
+            apply (lookup_weaken (<[ k := v]> sm)) ; last done.
+            apply lookup_insert_eq.
+          }
+          simpl.
+          wp_apply wp_interace_eq.
+          iIntros (b) "%Hb".
+          subst.
+          rewrite bool_decide_eq_true_2.
+          {
+            apply map_subseteq_spec.
+            intros ? ? Hlookup.
+            apply (lookup_weaken (<[ k := v]> sm)) ; last done.
+            apply lookup_insert_Some.
+            right.
+            split ; last done.
+            unfold not.
+            intros Heq.
+            apply Hk_not_elem_of_sm.
+            rewrite <- Heq in Hlookup.
+            apply (elem_of_dom_2 _ _ x).
+            done.
+          }
+          rewrite bool_decide_eq_true_2 ; first done.
+          wp_auto.
+          destruct (decide _) ; first done.
+          destruct (decide _).
+          {
+            apply (inj to_val) in e.
+            discriminate.
+          }
+          iPureIntro.
+          apply n.
+          reflexivity.
+        - unfold is_Some in i.
+          destruct i as [v' Hm2_lookup_k].
+          rewrite Hm2_lookup_k.
+          simpl.
+          wp_apply wp_interace_eq.
+          iIntros (b) "%Hb".
+          case_bool_decide.
+          + subst.
+            wp_auto.
+            destruct (decide _).
+            {
+              rewrite bool_decide_eq_false_2 ; last done.
+              unfold not.
+              intros Hsubset_eq.
+              apply n.
+              apply insert_subseteq_l ; done.
+            }
+            destruct (decide _).
+            {
+              apply (inj to_val) in e.
+              discriminate.
+            }
+            iPureIntro.
+            apply n0.
+            done.
+          + subst.
+            wp_auto.
+            destruct (decide _).
+            {
+              apply (inj to_val) in e.
+              discriminate.
+            }
+            destruct (decide _).
+            {
+              rewrite bool_decide_eq_false_2 ; last done.
+              unfold not.
+              intros Heq.
+              apply n.
+              rewrite <- Heq.
+              done.
+            }
+            iPureIntro.
+            apply n1.
+            reflexivity.
+      }
+      rewrite bool_decide_eq_false_2 ; last done.
+      unfold not.
+      intros Heq.
+      apply n.
+      rewrite <- Heq.
+      apply (lookup_weaken_is_Some (<[ k := v]> sm)) ; last done.
+      apply lookup_insert_is_Some.
+      left.
+      done.
+    }
+    iIntros "ret_val".
+    rewrite Hs2 in Hs1.
+    case_bool_decide.
+    - assert (m1 = m2).
+      {
+        apply map_subseteq_size_eq ; [done | lia].
+      }
+      rewrite bool_decide_eq_true_2 ; done.
+    - rewrite bool_decide_eq_false_2 ; [set_solver | done].
+  }
+  iIntros (?) "ret_val".
+  wp_auto.
+  iApply "HΦ".
+  done.
+Qed.
+
+End proof.
